Prove commutation lemma.

Trivalent.v
@@ -2,10 +2,11 @@ Inductive T :=
 | true : T
 | false : T.
 
-Definition T_elim {a : Type} (p : T) (v1 v2 : a) : a := match p with
-                                                        | true => v1
-                                                        | false => v2
-                                                        end.
+Definition T_elim {a : Type} (p : T) (v1 v2 : a) : a :=
+  match p with
+  | true => v1
+  | false => v2
+  end.
 
 Theorem T_not_eq : ~ (true = false).
 Proof.
@@ -20,24 +21,33 @@ Proof.
   exact u.
 Qed.
 
+Check T_not_eq.
+
 Inductive THash :=
 | trueHash : THash
 | falseHash : THash
 | hash : THash.
 
-Definition THash_elim {a : Type} (p : THash) (v1 v2 v3 : a) : a := match p with
-                                                               | trueHash => v1
-                                                               | falseHash => v2
-                                                               | hash => v3
-                                                               end.
+Print T_not_eq.
 
-Theorem THash_not_eq : ~ (trueHash = falseHash) /\ ~ (hash = trueHash) /\ ~ (hash = falseHash).
+Definition THash_elim {a : Type} (p : THash) (v1 v2 v3 : a) : a :=
+  match p with
+  | trueHash => v1
+  | falseHash => v2
+  | hash => v3
+  end.
+
+Theorem THash_not_eq : ~ (trueHash = falseHash) /\
+                         ~ (hash = trueHash) /\
+                         ~ (hash = falseHash).
 Proof.
   split.
   intro.
   pose (eq_refl (THash_elim trueHash unit False unit)).
-  replace (THash_elim trueHash unit False unit = THash_elim trueHash unit False unit) with
-    (THash_elim trueHash unit False unit = THash_elim falseHash unit False unit)
+  replace (THash_elim trueHash unit False unit =
+             THash_elim trueHash unit False unit) with
+    (THash_elim trueHash unit False unit =
+       THash_elim falseHash unit False unit)
     in e by now (rewrite H).
   pose tt.
   unfold THash_elim in e.
@@ -46,8 +56,10 @@ Proof.
   split.
   intro.
   pose (eq_refl (THash_elim trueHash unit unit False)).
-  replace (THash_elim trueHash unit unit False = THash_elim trueHash unit unit False) with
-    (THash_elim trueHash unit unit False = THash_elim hash unit unit False)
+  replace (THash_elim trueHash unit unit False =
+             THash_elim trueHash unit unit False) with
+    (THash_elim trueHash unit unit False =
+       THash_elim hash unit unit False)
     in e by now (rewrite H).
   pose tt.
   unfold THash_elim in e.
@@ -55,8 +67,10 @@ Proof.
   exact u.
   intro.
   pose (eq_refl (THash_elim falseHash unit unit False)).
-  replace (THash_elim falseHash unit unit False = THash_elim falseHash unit unit False) with
-    (THash_elim falseHash unit unit False = THash_elim hash unit unit False)
+  replace (THash_elim falseHash unit unit False =
+             THash_elim falseHash unit unit False) with
+    (THash_elim falseHash unit unit False =
+       THash_elim hash unit unit False)
     in e by now (rewrite H).
   pose tt.
   unfold THash_elim in e.
@@ -114,11 +128,17 @@ Proof.
   elim H4.
   intros.
   pose (existsHashDef1 (ex_intro (fun x0 : b => k (x1, x0) = trueHash) x0 H5)).
-  pose (existsHashDef1 (ex_intro (fun x1 : a => existsHash (fun x0 : b => k (x1, x0)) = trueHash) x1 e1)).
+  pose (existsHashDef1
+          (ex_intro (fun x1 : a =>
+                       existsHash (fun x0 : b =>
+                                     k (x1, x0)) = trueHash) x1 e1)).
   rewrite H in e2.
   exact (proj1 THash_not_eq (eq_sym e2)).
-  pose (ex_intro (fun x0 : b => existsHash (fun x1 : a => k (x1, x0)) = falseHash) x0 (existsHashDef2 (conj e0 H4))).
-  assert (not (exists x0 : b, existsHash (fun x1 : a => k (x1, x0)) = trueHash)).
+  pose (ex_intro (fun x0 : b =>
+                    existsHash (fun x1 : a => k (x1, x0)) = falseHash)
+          x0 (existsHashDef2 (conj e0 H4))).
+  assert (not
+            (exists x0 : b, existsHash (fun x1 : a => k (x1, x0)) = trueHash)).
   intro.
   elim H5.
   intros.
@@ -126,7 +146,10 @@ Proof.
   elim e2.
   intros.
   pose (existsHashDef1 (ex_intro (fun x1 : b => k (x2, x1) = trueHash) x1 H7)).
-  pose (existsHashDef1 (ex_intro (fun x2 : a => existsHash (fun x1 : b => k (x2, x1)) = trueHash) x2 e3)).
+  pose (existsHashDef1
+          (ex_intro (fun x2 : a =>
+                       existsHash (fun x1 :
+                                     b => k (x2, x1)) = trueHash) x2 e3)).
   rewrite H in e4.
   exact (proj1 THash_not_eq (eq_sym e4)).
   exact (eq_sym (existsHashDef2  (conj e1 H5))).
@@ -189,7 +212,7 @@ Proof.
   intro.
   trivial.
 Qed.
-   
+  
 Lemma andHash_assoc : forall (x y z : THash),
     andHash x (andHash y z) = andHash (andHash x y) z.
 Proof.
@@ -305,7 +328,7 @@ Proof.
   repeat rewrite (proj2 (andHashDef1 hash)). trivial.
 Qed.
  
-Lemma andHash_is_true : forall (x  y : THash),
+Lemma andHash_is_true : forall {x  y : THash},
     andHash x y = trueHash -> x = trueHash /\ y = trueHash.
 Proof.
   intros.
@@ -358,7 +381,7 @@ Proof.
   exact (conj H H).
 Qed.
 
-Lemma andHash_is_false1 : forall (x y : THash),
+Lemma andHash_is_false1 : forall {x y : THash},
     andHash x y = falseHash -> x = falseHash \/ y = falseHash.
 Proof.
   intros.
@@ -399,7 +422,7 @@ Proof.
   inversion f.
 Qed.
 
-Lemma andHash_is_false2 : forall (x y : THash),
+Lemma andHash_is_false2 : forall {x y : THash},
     andHash x y = falseHash ->
     (x = trueHash \/ x = falseHash) /\ (y = trueHash \/ y = falseHash).
 Proof.
@@ -421,7 +444,7 @@ Proof.
   exact (H y x H0).
 Qed.
  
-Lemma andHash_is_hash : forall (x y : THash),
+Lemma andHash_is_hash : forall {x y : THash},
     andHash x y = hash -> x = hash \/ y = hash.
 Proof.
   intros.
@@ -508,7 +531,7 @@ Proof.
   intros.
   case_eq (andHash (existsHash phi) p).
   intro.
-  pose (andHash_is_true (existsHash phi) p H).
+  pose (andHash_is_true H).
   pose (existsHashDef1' (proj1 a0)).
   elim e.
   intros.
@@ -521,7 +544,7 @@ Proof.
            (existsHashDef1
               (ex_intro (fun x0 : a => andHash (phi x0) p = trueHash) x e0))).
   intro.
-  pose (andHash_is_false1 (existsHash phi) p H).
+  pose (andHash_is_false1 H).
   elim o.
   intro.
   pose (existsHashDef2' H0).
@@ -551,7 +574,7 @@ Proof.
   intros.
   exact (proj2 a0 (ex_intro
                      (fun x => phi x = trueHash)
-                     x (proj1 (andHash_is_true (phi x) p H3)))).
+                     x (proj1 (andHash_is_true H3)))).
   exact (eq_sym (existsHashDef2 (conj H1 H2))).
   intro.
   rewrite H0.
@@ -564,7 +587,7 @@ Proof.
   assert (~ exists x : a, andHash (phi x) falseHash = trueHash). intro.
   elim H3. intros.
   exact (proj1 THash_not_eq
-           (eq_sym (proj2 (andHash_is_true (phi x0) falseHash H4)))).
+           (eq_sym (proj2 (andHash_is_true H4)))).
   exact (eq_sym (existsHashDef2 (conj e1 H3))).
   intro.
   pose (existsHashDef2' H1).
@@ -577,10 +600,10 @@ Proof.
   assert (~ exists x : a, andHash (phi x) falseHash = trueHash). intro.
   elim H3. intros.
   exact (proj1 THash_not_eq
-           (eq_sym (proj2 (andHash_is_true (phi x) falseHash H4)))).
+           (eq_sym (proj2 (andHash_is_true H4)))).
   exact (eq_sym (existsHashDef2 (conj H2 H3))).
   intro.
-  elim (proj1 (andHash_is_false2 (existsHash phi) p H)). intro.
+  elim (proj1 (andHash_is_false2 H)). intro.
   rewrite H1 in H2.
   pose (proj1 (proj2 THash_not_eq) H2).
   inversion f.
@@ -590,7 +613,7 @@ Proof.
   inversion f.
   intro.
   assert (forall x : a, andHash (phi x) p = hash). intro.
-  pose (andHash_is_hash (existsHash phi) p H).
+  pose (andHash_is_hash H).
   elim o. intro.
   pose (existsHashDef3' H0 x).
   pose (proj2 (andHashDef1 p)).
@@ -613,39 +636,186 @@ Lemma existsHash_andHash_existsHash_andHash : forall {a b : Set}
       existsHash (fun y : b =>
                     andHash (m y) (existsHash (fun x : a =>
                                                  andHash (n x y) (o x)))).
-Admitted.                       (* Taking forever *)
-(* Proof. *)
-(*   intros. *)
-(*   case_eq (existsHash (fun x : a => andHash (existsHash (fun y : b => andHash (m y) (n x y))) (o x))). intros. *)
-(*   pose (existsHashDef1' a (fun x : a => andHash (existsHash (fun y : b => andHash (m y) (n x y))) (o x)) H). *)
-(*   elim e. intros. *)
-(*   rewrite (andHash_existsHash_comm b (o x) (fun y : b => andHash (m y) (n x y))) in H0. *)
-(*   pose (existsHashDef1' b (fun x0 : b => andHash (andHash (m x0) (n x x0)) (o x)) H0). *)
-(*   elim e0. intros. *)
-(*   pose (andHash_is_true (andHash (m x0) (n x x0)) (o x) H1). *)
-(*   pose (andHash_is_true (m x0) (n x x0) (proj1 a0)). *)
-(*   assert (exists (x1 : a), andHash (n x1 x0) (o x1) = trueHash). *)
-(*   pose andHashDef3. *)
-(*   replace (andHash trueHash trueHash = trueHash) with (andHash (n x x0) trueHash = trueHash) in e1 by now (rewrite (proj2 a1)). *)
-(*   replace  (andHash (n x x0) trueHash = trueHash) with (andHash (n x x0) (o x) = trueHash) in e1 by now (rewrite (proj2 a0)). *)
-(*   exact (ex_intro (fun x1 : a => andHash (n x1 x0) (o x1) = trueHash) x e1). *)
-(*   pose (existsHashDef1 a (fun x1 : a => andHash (n x1 x0) (o x1)) H2). *)
-(*   pose andHashDef3. *)
-(*   replace (andHash trueHash trueHash = trueHash) with (andHash trueHash (existsHash (fun x1 : a => andHash (n x1 x0) (o x1))) = trueHash) in e2 by now (rewrite (eq_sym e1)). *)
-(*   replace (andHash trueHash (existsHash (fun x1 : a => andHash (n x1 x0) (o x1))) = trueHash) with (andHash (m x0) (existsHash (fun x1 : a => andHash (n x1 x0) (o x1))) = trueHash) in e2 by now (rewrite (eq_sym (proj1 a1))). *)
-(*   exact (eq_sym (existsHashDef1 b (fun y : b => andHash (m y) (existsHash (fun x1 : a => andHash (n x1 y) (o x1)))) (ex_intro (fun y : b => andHash (m y) (existsHash (fun x1 : a => andHash (n x1 y) (o x1))) = trueHash) x0 e2))). *)
-(*   intros. *)
-(*   pose (existsHashDef2' a (fun x : a => andHash (existsHash (fun y : b => andHash (m y) (n x y))) (o x)) H). *)
-(*   assert (exists (y : b),  andHash (m y) (existsHash (fun x : a => andHash (n x y) (o x))) = falseHash). *)
-(*   elim (proj1 a0). intros. *)
-(*   pose (andHash_is_false1 (existsHash (fun y : b => andHash (m y) (n x y))) (o x) H0). *)
-(*   elim o0. intro. *)
-(*   pose (existsHashDef2' b (fun y : b => andHash (m y) (n x y)) H1). *)
-(*   elim (proj1 a1). intros. *)
-(*   assert ((exists (x1 : a), andHash (n x1 x0) (o x1) = falseHash) /\ ~ exists (x1 : a), andHash (n x1 x0) (o x1) = trueHash). *)
-(*   split. *)
-(*   pose (andHash *)
-(*   exact (ex_intro (fun x1 : a => andHash (n x1 x0) (o x1) = falseHash) x H2). *)
+(* Admitted.                       (* Taking forever *) *)
+Proof.
+  intros.
+  case_eq (existsHash (fun x : a =>
+                         andHash (existsHash (fun y : b =>
+                                                andHash (m y)
+                                                  (n x y))) (o x))).
+  intros.
+  pose (existsHashDef1' H).
+  elim e. intros.
+  rewrite (andHash_existsHash_comm (fun y : b =>
+                                      andHash (m y) (n x y))) in H0.
+  pose (existsHashDef1' H0).
+  elim e0. intros.
+  pose (andHash_is_true H1).
+  pose (andHash_is_true (proj1 a0)).
+  assert (exists (x1 : a), andHash (n x1 x0) (o x1) = trueHash).
+  pose andHashDef3.
+  replace (andHash trueHash trueHash = trueHash) with
+    (andHash (n x x0) trueHash = trueHash) in e1 by now (rewrite (proj2 a1)).
+  replace  (andHash (n x x0) trueHash = trueHash) with
+    (andHash (n x x0) (o x) = trueHash) in e1 by now (rewrite (proj2 a0)).
+  exact (ex_intro (fun x1 : a => andHash (n x1 x0) (o x1) = trueHash) x e1).
+  pose (existsHashDef1 H2).
+  pose andHashDef3.
+  replace (andHash trueHash trueHash = trueHash) with
+    (andHash trueHash (existsHash (fun x1 : a =>
+                                     andHash (n x1 x0) (o x1))) = trueHash)
+    in e2 by now (rewrite (eq_sym e1)).
+  replace (andHash trueHash (existsHash (fun x1 : a =>
+                                           andHash (n x1 x0)
+                                             (o x1))) = trueHash) with
+    (andHash (m x0) (existsHash (fun x1 : a =>
+                                   andHash (n x1 x0) (o x1))) = trueHash)
+    in e2 by now (rewrite (eq_sym (proj1 a1))).
+  exact (eq_sym
+           (existsHashDef1 (ex_intro (fun y : b =>
+                                        andHash (m y)
+                                          (existsHash (fun x1 : a =>
+                                                         andHash (n x1 y)
+                                                           (o x1))) =
+                                          trueHash)
+                              x0 e2))).
+  intro.
+  case_eq (existsHash (fun y : b =>
+                         andHash (m y)
+                           (existsHash (fun x : a => andHash (n x y) (o x))))).
+  intro.
+  pose (existsHashDef1' H0).
+  elim e. intros.
+  pose (andHash_is_true H1).
+  pose (existsHashDef1' (proj2 a0)).
+  elim e0. intros.
+  pose (andHash_is_true H2).
+  pose andHashDef3.
+  replace (andHash trueHash) with
+    (andHash (m x)) in e1 by now (rewrite (eq_sym (proj1 a0))).
+  replace (andHash (m x) trueHash) with
+    (andHash (m x) (n x0 x)) in e1 by now (rewrite (eq_sym (proj1 a1))).
+  pose (existsHashDef1 (ex_intro (fun y : b =>
+                                    andHash (m y) (n x0 y) = trueHash) x e1)).
+  pose andHashDef3.
+  replace (andHash trueHash) with
+    (andHash (existsHash (fun y : b => andHash (m y) (n x0 y)))) in e3 by
+      now (rewrite (eq_sym e2)).
+  replace (andHash (existsHash (fun y : b =>
+                                  andHash (m y) (n x0 y))) trueHash) with
+    (andHash (existsHash (fun y : b =>
+                            andHash (m y) (n x0 y))) (o x0))
+    in e3 by
+      now (rewrite (eq_sym (proj2 a1))).
+  rewrite (existsHashDef1
+             (ex_intro
+                (fun x : a =>
+                   andHash (existsHash
+                              (fun y : b =>
+                                 andHash (m y) (n x y))) (o x) = trueHash)
+                x0 e3)) in H.
+  exact (eq_sym H).
+  trivial.
+  intro.
+  assert (forall x : a,
+             andHash (existsHash (fun y : b =>
+                                    andHash (m y) (n x y))) (o x) = hash).
+  intro.
+  pose (existsHashDef3' H0).
+  case_eq (existsHash (fun y : b => andHash (m y) (n x y))). intro.
+  pose (existsHashDef1' H1).
+  elim e0. intros.
+  pose (andHash_is_hash (e x0)). elim o0. intro.
+  rewrite H3 in H2.
+  rewrite (proj2 (andHashDef1 (n x x0))) in H2.
+  pose (proj1 (proj2 THash_not_eq) H2).
+  inversion f.
+  intro.
+  pose (existsHashDef3' H3 x).
+  rewrite (eq_sym (proj2 (andHash_is_true H2))).
+  exact e1.
+  intro.
+  pose (existsHashDef2' H1).
+  elim (proj1 a0). intros.
+  pose (andHash_is_hash (e x0)). elim o0. intro.
+  rewrite H3 in H2.
+  rewrite (proj2 (andHashDef1 (n x x0))) in H2.
+  pose (proj2 (proj2 THash_not_eq) H2).
+  inversion f.
+  intro.
+  elim (andHash_is_hash (existsHashDef3' H3 x)). intro.
+  rewrite H4 in H2.
+  rewrite (proj1 (andHashDef1 (m x0))) in H2.
+  pose (proj2 (proj2 THash_not_eq) H2).
+  inversion f.
+  intro.
+  rewrite H4.
+  apply (proj1 (andHashDef1 falseHash)).
+  intro.
+  apply (proj2 (andHashDef1 (o x))).
+  pose (existsHashDef2' H).
+  elim (proj1 a0). intros.
+  elim (andHash_is_hash (H1 x)). intro.
+  elim (proj1 (andHash_is_false2 H2)).
+  rewrite H3.
+  intro.
+  pose (proj1 (proj2 THash_not_eq) H4).
+  inversion f.
+  intro.
+  rewrite H4 in H3.
+  exact H3.
+  intro.
+  rewrite H3 in H2.
+  rewrite (proj1 (andHashDef1 (existsHash (fun y : b =>
+                                             andHash (m y) (n x y))))) in H2.
+  exact (eq_sym H2).
+  intro.
+  assert (forall (y : b),
+             andHash (m y)
+               (existsHash (fun x : a =>
+                              andHash (n x y) (o x))) = hash). intro.
+  case_eq (m y). intro.
+  assert (forall (x : a), andHash (n x y) (o x) = hash). intro.
+  pose (existsHashDef3' H x).
+  pose (andHash_is_hash e).
+  elim o0. intro.
+  pose (existsHashDef3' H1 y).
+  pose (andHash_is_hash e0).
+  elim o1. intro.
+  rewrite H0 in H2.
+  pose (proj1 (proj2 THash_not_eq) (eq_sym H2)).
+  inversion f.
+  intro.
+  rewrite H2.
+  exact (proj2 (andHashDef1 (o x))).
+  intro.
+  rewrite H1.
+  exact (proj1 (andHashDef1 (n x y))).
+  rewrite (existsHashDef3 H1).
+  exact (proj1 (andHashDef1 trueHash)).
+  intro.
+    assert (forall (x : a), andHash (n x y) (o x) = hash). intro.
+  pose (existsHashDef3' H x).
+  pose (andHash_is_hash e).
+  elim o0. intro.
+  pose (existsHashDef3' H1 y).
+  pose (andHash_is_hash e0).
+  elim o1. intro.
+  rewrite H0 in H2.
+  pose (proj2 (proj2 THash_not_eq) (eq_sym H2)).
+  inversion f.
+  intro.
+  rewrite H2.
+  exact (proj2 (andHashDef1 (o x))).
+  intro.
+  rewrite H1.
+  exact (proj1 (andHashDef1 (n x y))).
+  rewrite (existsHashDef3 H1).
+  exact (proj1 (andHashDef1 falseHash)).
+  intro.
+  exact (proj2 (andHashDef1 (existsHash (fun x : a => andHash (n x y) (o x))))).
+  exact (eq_sym (existsHashDef3 H0)).
+Qed.
   
 Lemma delt_true : forall {x : T}, delt x = trueHash -> x = true.
 Proof.
@@ -740,7 +910,7 @@ Proof.
   intro.
   elim H0.
   intros.
-  pose (andHash_is_true (delt (eqHash x v)) (phi x) H1).
+  pose (andHash_is_true H1).
   pose (proj1 a0).
   pose (eqHashRefl2 (delt_true e2)).
   pose (proj2 a0).
@@ -818,12 +988,23 @@ Proof.
   split.
   unfold monad_right_id. unfold bindHash. unfold etaHash.
   intros.
-  pose (functional_extensionality (fun y : a => existsHash (fun x : a => andHash (m' x) (delt (eqHash y x)))) m').
-  assert (forall x : a, existsHash (fun x0 : a => andHash (m' x0) (delt (eqHash x x0))) = m' x).
+  pose (functional_extensionality
+          (fun y : a =>
+             existsHash (fun x : a => andHash (m' x) (delt (eqHash y x)))) m').
+  assert (forall x : a,
+             existsHash (fun x0 : a =>
+                           andHash (m' x0) (delt (eqHash x x0))) = m' x).
   intro.
-  assert ((fun x0 : a => andHash (m' x0) (delt (eqHash x x0))) = fun x0 : a => andHash (delt (eqHash x0 x)) (m' x0)).
-  pose (functional_extensionality (fun x0 : a => andHash (m' x0) (delt (eqHash x x0))) (fun x0 : a => andHash (delt (eqHash x0 x)) (m' x0))).
-  assert (forall x0 : a, andHash (m' x0) (delt (eqHash x x0)) = andHash (delt (eqHash x0 x)) (m' x0)).
+  assert ((fun x0 : a => andHash (m' x0) (delt (eqHash x x0))) =
+            fun x0 : a => andHash (delt (eqHash x0 x)) (m' x0)).
+  pose (functional_extensionality
+          (fun x0 : a =>
+             andHash (m' x0)
+               (delt (eqHash x x0))) (fun x0 : a =>
+                                        andHash (delt (eqHash x0 x)) (m' x0))).
+  assert (forall x0 : a,
+             andHash (m' x0)
+               (delt (eqHash x x0)) = andHash (delt (eqHash x0 x)) (m' x0)).
   intro.
   rewrite (eqHash_comm x x0).
   exact (andHash_comm (m' x0) (delt (eqHash x0 x))).
@@ -833,9 +1014,32 @@ Proof.
   exact (e H).
   unfold monad_assoc. unfold bindHash.
   intros.
-  pose (functional_extensionality  (fun y : c => existsHash (fun x : b => andHash (existsHash (fun x0 : a => andHash (m' x0) (n x0 x))) (o x y))) (fun y : c => existsHash (fun x : a => andHash (m' x) (existsHash (fun x0 : b => andHash (n x x0) (o x0 y)))))).
-  assert (forall x : c, existsHash (fun x0 : b => andHash (existsHash (fun x1 : a => andHash (m' x1) (n x1 x0))) (o x0 x)) = existsHash (fun x0 : a => andHash (m' x0) (existsHash (fun x1 : b => andHash (n x0 x1) (o x1 x))))). intro.
-  exact (existsHash_andHash_existsHash_andHash m' (fun x y => n y x) (fun x1 => o x1 x)).
+  pose (functional_extensionality
+          (fun y : c =>
+             existsHash (fun x : b =>
+                           andHash
+                             (existsHash (fun x0 : a =>
+                                            andHash (m' x0)
+                                              (n x0 x))) (o x y)))
+          (fun y : c =>
+             existsHash (fun x : a =>
+                           andHash (m' x)
+                             (existsHash (fun x0 : b =>
+                                            andHash (n x x0) (o x0 y)))))).
+  assert (forall x : c,
+             existsHash (fun x0 : b =>
+                           andHash (existsHash (fun x1 : a =>
+                                                  andHash (m' x1)
+                                                    (n x1 x0))) (o x0 x)) =
+               existsHash (fun x0 : a =>
+                             andHash (m' x0)
+                               (existsHash (fun x1 : b =>
+                                              andHash (n x0 x1)
+                                                (o x1 x))))).
+  intro.
+  exact (existsHash_andHash_existsHash_andHash
+           m' (fun x y => n y x) (fun x1 => o x1 x)).
   apply functional_extensionality. intro.
-  exact (existsHash_andHash_existsHash_andHash m' (fun x y => n y x) (fun x1 => o x1 x)).
+  exact (existsHash_andHash_existsHash_andHash
+           m' (fun x y => n y x) (fun x1 => o x1 x)).
 Qed.
